subgraph.v
@@ -1,0 +1,166 @@
+Require Import graph.
+Require Import List.
+Require Import Setoid.  (* Generalized rewriting *)
+Require Import FSets.   (* Efficient functional sets *)
+Require Import FMaps.   (* Efficient functional maps *)
+Require Import PArith.
+From Hammer Require Import Hammer.
+From Hammer Require Import Tactics.
+Import Arith.
+Import ListNotations.
+Import Nat.
+
+(* The neighbors of a vertex v in a graph g. *)
+Definition neighbors (g : graph) v := adj g v.
+
+(* Subgraph induced by a set of vertices *)
+Definition subgraph_of (g : graph) (s : S.t) :=
+  M.fold (fun v adj g' => if S.mem v s then M.add v (S.filter (fun u => S.mem u s) adj) g' else g') g empty_graph.
+
+(* g' is a subgraph of g if:
+- the vertex set of g' is a subset of the vertex set of g
+- for every vertex v in g', the 
+ *)
+Definition is_subgraph (g' g : graph) :=
+  (S.Subset (nodes g') (nodes g)) /\ (forall v, S.Subset (adj g' v) (adj g v)).
+
+
+
+(* Some lemmas about induced subgraphs. *)
+(* The nodes of a subgraph are a subset of the original graph. *)
+Lemma subgraph_vertices : forall g s, S.Subset (nodes (subgraph_of g s)) (nodes g).
+Proof.
+  intros g s.
+  unfold subgraph_of.
+  apply WP.fold_rec_bis.
+  - intros m m' a H H0.
+    sauto unfold: M.In, M.MapsTo, nodes, S.Subset use: Sin_domain.
+  - sfirstorder.
+  - intros k e a m' H H0 H1.
+    intros a' Ha'.
+    sdestruct (S.mem k s).
+    + destruct (E.eq_dec a' k).
+      * subst.
+        unfold nodes.
+        apply Sin_domain.
+        hauto lq: on rew: off use: WF.add_in_iff.
+      * unfold nodes in *.
+        unfold S.Subset in H1.
+        assert (S.In a' (Mdomain m')).
+        {
+          hauto l: on use: WP.F.add_neq_in_iff, Sin_domain.
+        }
+        hauto lq: on rew: off use: WP.F.add_neq_in_iff, Sin_domain.
+    + apply H1 in Ha'.
+      apply Sin_domain.
+      apply Sin_domain in Ha'.
+      destruct (E.eq_dec a' k); sauto lq: on rew: off use: WP.F.add_neq_in_iff.
+Qed.
+
+
+(* The edges of a subgraph are a subset of the original graph. *)
+(* Note this is defined pointwise: the adjacency set is a subset for every vertex. *)
+Lemma subgraph_edges : forall g s v,
+    S.Subset (adj (subgraph_of g s) v) (adj g v).
+Proof.
+  intros g s v.
+  unfold subgraph_of.
+  apply WP.fold_rec_bis.
+  - intros m m' a H1 H2.
+    unfold adj, nodeset in *.
+    unfold nodeset in *.
+    hauto drew: off.
+  - sfirstorder.
+  - intros k e a m' H1 H2 H3.
+    (* k is the node we're considering to add to the new subgraph *)
+    sdestruct (S.mem k s).
+    + (* suppose it's in the set *)
+      unfold adj.
+      intros a' Ha'.
+      destruct (E.eq_dec v k).
+      * subst.
+        unfold nodeset in *.
+        rewrite PositiveMap.gss in *.
+        strivial use: PositiveSet.xfilter_spec unfold: PositiveSet.elt, PositiveSet.filter.
+      * rewrite PositiveMap.gso in *; auto.
+    + (* suppose it's not in the set *)
+      ssimpl.
+      unfold S.Subset in *.
+      intros a' Ha'.
+      specialize (H3 a').
+      unfold adj in *.
+      destruct (E.eq_dec v k).
+      * fcrush.
+      * apply H3 in Ha'.
+        assert (M.find v (M.add k e m') = M.find v m').
+        {
+          hauto lq: on rew: off use: PositiveMap.gso unfold: PositiveSet.elt, PositiveMap.key.
+        }
+        unfold nodeset in *.
+        hauto lq: on.
+Qed.
+
+Lemma subgraph_of_is_subgraph : forall g s, is_subgraph (subgraph_of g s) g.
+Proof.
+  intros g s.
+  unfold is_subgraph.
+  split; [apply subgraph_vertices|apply subgraph_edges].
+Qed.
+
+(* The (open) neighborhood of a vertex v in a graph consists of the
+   subgraph induced by the vertices adjacent to v.  It does not
+   include v itself. *)
+Definition neighborhood (g : graph) v := remove_node v (subgraph_of g (neighbors g v)).
+
+(* Neighborhoods do not include their vertex *)
+Lemma nbd_not_include_vertex g v : M.find v (neighborhood g v) = None.
+Proof.
+  hecrush use: WF.map_o use: M.grs.
+Qed.
+
+(* A subgraph of an undirected graph is undirected *)
+Lemma subgraph_undirected : forall g g', undirected g -> is_subgraph g' g -> undirected g'.
+Proof.
+  intros g g' H H0.
+  unfold undirected.
+  intros i j Ug.
+  assert (S.In j (adj g i)).
+  {
+    sfirstorder.
+  }
+  assert (S.In i (adj g j)).
+  {
+    hauto l: on.
+  }
+Admitted.
+  
+(* A subgraph of a graph is colorable under the same coloring *)
+Lemma subgraph_colorable : forall (g g' : graph) f p,
+    undirected g ->
+    is_subgraph g' g ->
+    coloring_ok p g f ->
+    coloring_ok p g' f.
+Proof.
+  intros g g' f p H H0 H1.
+  hfcrush use: subgraph_of_is_subgraph unfold: is_subgraph, PositiveSet.Subset, coloring_ok, undirected.
+Qed.
+
+Definition remove_subgraph (g : graph) s :=
+  M.fold (fun v e m' => if S.mem v s then m' else M.add v (S.diff e s) m') (@M.empty _) g.
+
+Lemma remove_subgraph_is_subgraph : forall g s, is_subgraph (remove_subgraph g s) g.
+Proof.
+  intros g s.
+  split.
+  - unfold remove_subgraph.
+    apply WP.fold_rec_bis.
+    + hauto lq: on.
+    + scongruence.
+    + sauto q: on.
+  - unfold remove_subgraph.
+    apply WP.fold_rec_bis.
+    + hauto lq: on.
+    + scongruence.
+    + intros k e a m' H H0 H1 v.
+      sauto q: on.
+Qed.
